Add BUpdFacts and FUpdFacts.

theories/bi/updates.v
@@ -1,7 +1,7 @@
 From stdpp Require Import coPset.
-From iris.bi Require Import interface.
+From iris.bi Require Import interface derived_laws big_op.
 
-Class BUpd (A : Type) : Type := bupd : A → A.
+Class BUpd (PROP : Type) : Type := bupd : PROP → PROP.
 Instance : Params (@bupd) 2.
 
 Notation "|==> Q" := (bupd Q)
@@ -11,7 +11,7 @@ Notation "P ==∗ Q" := (P ⊢ |==> Q)
 Notation "P ==∗ Q" := (P -∗ |==> Q)%I
   (at level 99, Q at level 200, format "P  ==∗  Q") : bi_scope.
 
-Class FUpd (A : Type) : Type := fupd : coPset → coPset → A → A.
+Class FUpd (PROP : Type) : Type := fupd : coPset → coPset → PROP → PROP.
 Instance: Params (@fupd) 4.
 
 Notation "|={ E1 , E2 }=> Q" := (fupd E1 E2 Q)
@@ -46,3 +46,174 @@ Notation "|={ E }▷=> Q" := (|={E,E}▷=> Q)%I
 Notation "P ={ E }▷=∗ Q" := (P ={E,E}▷=∗ Q)%I
   (at level 99, E at level 50, Q at level 200,
    format "P  ={ E }▷=∗  Q") : bi_scope.
+
+(** BUpd facts  *)
+
+Class BUpdFacts (PROP : bi) `{BUpd PROP} : Prop :=
+  { bupd_ne :> NonExpansive bupd;
+    bupd_intro P : P ==∗ P;
+    bupd_mono P Q : (P ⊢ Q) → (|==> P) ==∗ Q;
+    bupd_trans P : (|==> |==> P) ==∗ P;
+    bupd_frame_r P R : (|==> P) ∗ R ==∗ P ∗ R;
+    bupd_plainly P : (|==> bi_plainly P) -∗ P }.
+
+Section bupd_derived.
+  Context `{BUpdFacts PROP}.
+
+  Global Instance bupd_proper : Proper ((≡) ==> (≡)) bupd := ne_proper _.
+
+  (** BUpd derived rules *)
+
+  Global Instance bupd_mono' : Proper ((⊢) ==> (⊢)) bupd.
+  Proof. intros P Q; apply bupd_mono. Qed.
+  Global Instance bupd_flip_mono' : Proper (flip (⊢) ==> flip (⊢)) bupd.
+  Proof. intros P Q; apply bupd_mono. Qed.
+
+  Lemma bupd_frame_l R Q : (R ∗ |==> Q) ==∗ R ∗ Q.
+  Proof. rewrite !(comm _ R); apply bupd_frame_r. Qed.
+  Lemma bupd_wand_l P Q : (P -∗ Q) ∗ (|==> P) ==∗ Q.
+  Proof. by rewrite bupd_frame_l bi.wand_elim_l. Qed.
+  Lemma bupd_wand_r P Q : (|==> P) ∗ (P -∗ Q) ==∗ Q.
+  Proof. by rewrite bupd_frame_r bi.wand_elim_r. Qed.
+  Lemma bupd_sep P Q : (|==> P) ∗ (|==> Q) ==∗ P ∗ Q.
+  Proof. by rewrite bupd_frame_r bupd_frame_l bupd_trans. Qed.
+  Lemma bupd_affinely_plainly `{BiAffine PROP} P : (|==> ■ P) ⊢ P.
+  Proof. by rewrite bi.affine_affinely bupd_plainly. Qed.
+  Lemma bupd_plain P `{!Plain P} : (|==> P) ⊢ P.
+  Proof. by rewrite {1}(plain P) bupd_plainly. Qed.
+End bupd_derived.
+
+Lemma except_0_bupd {PROP : sbi} `{BUpdFacts PROP} (P : PROP) :
+  ◇ (|==> P) ⊢ (|==> ◇ P).
+Proof.
+  rewrite /sbi_except_0. apply bi.or_elim; eauto using bupd_mono, bi.or_intro_r.
+  by rewrite -bupd_intro -bi.or_intro_l.
+Qed.
+
+(** FUpd facts  *)
+
+(* Currently, this requires an SBI, because of [except_0_fupd] and
+   [later_fupd_plain]. If need be, we can generalize this to BIs by
+   extracting these propertes as lemmas to be proved by hand. *)
+Class FUpdFacts (PROP : sbi) `{BUpd PROP, FUpd PROP} : Prop :=
+  { fupd_bupd_facts :> BUpdFacts PROP;
+    fupd_ne E1 E2 :> NonExpansive (fupd E1 E2);
+    fupd_intro_mask E1 E2 P : E2 ⊆ E1 → P ⊢ |={E1,E2}=> |={E2,E1}=> P;
+    bupd_fupd E P : (|==> P) ={E}=∗ P;
+    except_0_fupd E1 E2 P : ◇ (|={E1,E2}=> P) ={E1,E2}=∗ P;
+    fupd_mono E1 E2 P Q : (P ⊢ Q) → (|={E1,E2}=> P) ⊢ |={E1,E2}=> Q;
+    fupd_trans E1 E2 E3 P : (|={E1,E2}=> |={E2,E3}=> P) ⊢ |={E1,E3}=> P;
+    fupd_mask_frame_r' E1 E2 Ef P :
+      E1 ## Ef → (|={E1,E2}=> ⌜E2 ## Ef⌝ → P) ={E1 ∪ Ef,E2 ∪ Ef}=∗ P;
+    fupd_frame_r E1 E2 P Q : (|={E1,E2}=> P) ∗ Q ={E1,E2}=∗ P ∗ Q;
+    fupd_plain' E1 E2 E2' P Q `{!Plain P} :
+      E1 ⊆ E2 →
+      (Q ={E1, E2'}=∗ P) -∗ (|={E1, E2}=> Q) ={E1}=∗ (|={E1, E2}=> Q) ∗ P;
+    later_fupd_plain E P `{!Plain P} : (▷ |={E}=> P) ={E}=∗ ▷ ◇ P }.
+
+Section fupd_derived.
+  Context `{FUpdFacts PROP}.
+
+  Global Instance fupd_proper E1 E2 : Proper ((≡) ==> (≡)) (fupd E1 E2) := ne_proper _.
+
+  (** FUpd derived rules *)
+
+  Global Instance fupd_mono' E1 E2 : Proper ((⊢) ==> (⊢)) (fupd E1 E2).
+  Proof. intros P Q; apply fupd_mono. Qed.
+  Global Instance fupd_flip_mono' E1 E2 :
+    Proper (flip (⊢) ==> flip (⊢)) (fupd E1 E2).
+  Proof. intros P Q; apply fupd_mono. Qed.
+
+  Lemma fupd_intro E P : P ={E}=∗ P.
+  Proof. rewrite -bupd_fupd. apply bupd_intro. Qed.
+  Lemma fupd_intro_mask' E1 E2 : E2 ⊆ E1 → (|={E1,E2}=> |={E2,E1}=> emp)%I.
+  Proof. exact: fupd_intro_mask. Qed.
+  Lemma fupd_except_0 E1 E2 P : (|={E1,E2}=> ◇ P) ={E1,E2}=∗ P.
+  Proof. by rewrite {1}(fupd_intro E2 P) except_0_fupd fupd_trans. Qed.
+
+  Lemma fupd_frame_l E1 E2 P Q : (P ∗ |={E1,E2}=> Q) ={E1,E2}=∗ P ∗ Q.
+  Proof. rewrite !(comm _ P); apply fupd_frame_r. Qed.
+  Lemma fupd_wand_l E1 E2 P Q : (P -∗ Q) ∗ (|={E1,E2}=> P) ={E1,E2}=∗ Q.
+  Proof. by rewrite fupd_frame_l bi.wand_elim_l. Qed.
+  Lemma fupd_wand_r E1 E2 P Q : (|={E1,E2}=> P) ∗ (P -∗ Q) ={E1,E2}=∗ Q.
+  Proof. by rewrite fupd_frame_r bi.wand_elim_r. Qed.
+
+  Lemma fupd_trans_frame E1 E2 E3 P Q :
+    ((Q ={E2,E3}=∗ emp) ∗ |={E1,E2}=> (Q ∗ P)) ={E1,E3}=∗ P.
+  Proof.
+    rewrite fupd_frame_l assoc -(comm _ Q) bi.wand_elim_r.
+    by rewrite fupd_frame_r left_id fupd_trans.
+  Qed.
+
+  Lemma fupd_mask_frame_r E1 E2 Ef P :
+    E1 ## Ef → (|={E1,E2}=> P) ={E1 ∪ Ef,E2 ∪ Ef}=∗ P.
+  Proof.
+    intros ?. rewrite -fupd_mask_frame_r' //. f_equiv.
+    apply bi.impl_intro_l, bi.and_elim_r.
+  Qed.
+  Lemma fupd_mask_mono E1 E2 P : E1 ⊆ E2 → (|={E1}=> P) ={E2}=∗ P.
+  Proof.
+    intros (Ef&->&?)%subseteq_disjoint_union_L. by apply fupd_mask_frame_r.
+  Qed.
+
+  Lemma fupd_sep E P Q : (|={E}=> P) ∗ (|={E}=> Q) ={E}=∗ P ∗ Q.
+  Proof. by rewrite fupd_frame_r fupd_frame_l fupd_trans. Qed.
+  Lemma fupd_big_sepL {A} E (Φ : nat → A → PROP) (l : list A) :
+    ([∗ list] k↦x ∈ l, |={E}=> Φ k x) ={E}=∗ [∗ list] k↦x ∈ l, Φ k x.
+  Proof.
+    apply (big_opL_forall (λ P Q, P ={E}=∗ Q)); auto using fupd_intro.
+    intros P1 P2 HP Q1 Q2 HQ. by rewrite HP HQ -fupd_sep.
+  Qed.
+  Lemma fupd_big_sepM `{Countable K} {A} E (Φ : K → A → PROP) (m : gmap K A) :
+    ([∗ map] k↦x ∈ m, |={E}=> Φ k x) ={E}=∗ [∗ map] k↦x ∈ m, Φ k x.
+  Proof.
+    apply (big_opM_forall (λ P Q, P ={E}=∗ Q)); auto using fupd_intro.
+    intros P1 P2 HP Q1 Q2 HQ. by rewrite HP HQ -fupd_sep.
+  Qed.
+  Lemma fupd_big_sepS `{Countable A} E (Φ : A → PROP) X :
+    ([∗ set] x ∈ X, |={E}=> Φ x) ={E}=∗ [∗ set] x ∈ X, Φ x.
+  Proof.
+    apply (big_opS_forall (λ P Q, P ={E}=∗ Q)); auto using fupd_intro.
+    intros P1 P2 HP Q1 Q2 HQ. by rewrite HP HQ -fupd_sep.
+  Qed.
+
+  Lemma fupd_plain E1 E2 P Q `{!Plain P} :
+    E1 ⊆ E2 → (Q -∗ P) -∗ (|={E1, E2}=> Q) ={E1}=∗ (|={E1, E2}=> Q) ∗ P.
+  Proof.
+    intros HE. rewrite -(fupd_plain' _ _ E1) //. apply bi.wand_intro_l.
+    by rewrite bi.wand_elim_r -fupd_intro.
+  Qed.
+
+  (** Fancy updates that take a step derived rules. *)
+
+  Lemma step_fupd_wand E1 E2 P Q : (|={E1,E2}▷=> P) -∗ (P -∗ Q) -∗ |={E1,E2}▷=> Q.
+  Proof.
+    apply bi.wand_intro_l.
+    by rewrite (bi.later_intro (P -∗ Q)%I) fupd_frame_l -bi.later_sep fupd_frame_l
+               bi.wand_elim_l.
+  Qed.
+
+  Lemma step_fupd_mask_frame_r E1 E2 Ef P :
+    E1 ## Ef → E2 ## Ef → (|={E1,E2}▷=> P) ⊢ |={E1 ∪ Ef,E2 ∪ Ef}▷=> P.
+  Proof.
+    intros. rewrite -fupd_mask_frame_r //. do 2 f_equiv. by apply fupd_mask_frame_r.
+  Qed.
+
+  Lemma step_fupd_mask_mono E1 E2 F1 F2 P :
+    F1 ⊆ F2 → E1 ⊆ E2 → (|={E1,F2}▷=> P) ⊢ |={E2,F1}▷=> P.
+  Proof.
+    intros ??. rewrite -(left_id emp%I _ (|={E1,F2}▷=> P)%I).
+    rewrite (fupd_intro_mask E2 E1 emp%I) //.
+    rewrite fupd_frame_r -(fupd_trans E2 E1 F1). f_equiv.
+    rewrite fupd_frame_l -(fupd_trans E1 F2 F1). f_equiv.
+    rewrite (fupd_intro_mask F2 F1 (|={_,_}=> emp)%I) //.
+    rewrite fupd_frame_r. f_equiv.
+    rewrite [X in (X ∗ _)%I]bi.later_intro -bi.later_sep. f_equiv.
+    rewrite fupd_frame_r -(fupd_trans F1 F2 E2). f_equiv.
+    rewrite fupd_frame_l -(fupd_trans F2 E1 E2). f_equiv.
+    by rewrite fupd_frame_r left_id.
+  Qed.
+
+  Lemma step_fupd_intro E1 E2 P : E2 ⊆ E1 → ▷ P -∗ |={E1,E2}▷=> P.
+  Proof. intros. by rewrite -(step_fupd_mask_mono E2 _ _ E2) // -!fupd_intro. Qed.
+End fupd_derived.
