theories/base_logic/lib/fancy_updates.v
@@ -13,237 +13,32 @@ Definition uPred_fupd_aux `{invG Σ} : seal uPred_fupd_def. by eexists. Qed.
 Instance uPred_fupd `{invG Σ} : FUpd (iProp Σ):= unseal uPred_fupd_aux.
 Definition uPred_fupd_eq `{invG Σ} : fupd = uPred_fupd_def := seal_eq uPred_fupd_aux.
 
-Section fupd.
-Context `{invG Σ}.
-Implicit Types P Q : iProp Σ.
-
-Global Instance fupd_ne E1 E2 : NonExpansive (fupd E1 E2).
-Proof. rewrite uPred_fupd_eq. solve_proper. Qed.
-Global Instance fupd_proper E1 E2 : Proper ((≡) ==> (≡)) (fupd E1 E2).
-Proof. apply ne_proper, _. Qed.
-
-Lemma fupd_intro_mask E1 E2 P : E2 ⊆ E1 → P ⊢ |={E1,E2}=> |={E2,E1}=> P.
+Instance fupd_facts `{invG Σ} : FUpdFacts (uPredSI (iResUR Σ)).
 Proof.
-  intros (E1''&->&?)%subseteq_disjoint_union_L.
-  rewrite uPred_fupd_eq /uPred_fupd_def ownE_op //.
-  by iIntros "$ ($ & $ & HE) !> !> [$ $] !> !>" .
+  split.
+  - apply _.
+  - rewrite uPred_fupd_eq. solve_proper.
+  - intros E1 E2 P (E1''&->&?)%subseteq_disjoint_union_L.
+    rewrite uPred_fupd_eq /uPred_fupd_def ownE_op //.
+      by iIntros "$ ($ & $ & HE) !> !> [$ $] !> !>" .
+  - rewrite uPred_fupd_eq. by iIntros (E P) ">? [$ $] !> !>".
+  - rewrite uPred_fupd_eq. iIntros (E1 E2 P) ">H [Hw HE]". iApply "H"; by iFrame.
+  - rewrite uPred_fupd_eq. iIntros (E1 E2 P Q HPQ) "HP HwE". rewrite -HPQ. by iApply "HP".
+  - rewrite uPred_fupd_eq. iIntros (E1 E2 E3 P) "HP HwE".
+    iMod ("HP" with "HwE") as ">(Hw & HE & HP)". iApply "HP"; by iFrame.
+  - intros E1 E2 Ef P HE1Ef. rewrite uPred_fupd_eq /uPred_fupd_def ownE_op //.
+    iIntros "Hvs (Hw & HE1 &HEf)".
+    iMod ("Hvs" with "[Hw HE1]") as ">($ & HE2 & HP)"; first by iFrame.
+    iDestruct (ownE_op' with "[HE2 HEf]") as "[? $]"; first by iFrame.
+    iIntros "!> !>". by iApply "HP".
+  - rewrite uPred_fupd_eq /uPred_fupd_def. by iIntros (????) "[HwP $]".
+  - iIntros (E1 E2 E2' P Q ? (E3&->&HE)%subseteq_disjoint_union_L) "HQP HQ".
+    rewrite uPred_fupd_eq /uPred_fupd_def ownE_op //. iIntros "H".
+    iMod ("HQ" with "H") as ">(Hws & [HE1 HE3] & HQ)"; iModIntro.
+    iAssert (◇ P)%I as "#HP".
+    { by iMod ("HQP" with "HQ [$]") as "(_ & _ & HP)". }
+    iMod "HP". iFrame. auto.
+  - rewrite uPred_fupd_eq /uPred_fupd_def. iIntros (E P ?) "HP [Hw HE]".
+    iAssert (▷ ◇ P)%I with "[-]" as "#$"; last by iFrame.
+    iNext. by iMod ("HP" with "[$]") as "(_ & _ & HP)".
 Qed.
-
-Lemma except_0_fupd E1 E2 P : ◇ (|={E1,E2}=> P) ={E1,E2}=∗ P.
-Proof. rewrite uPred_fupd_eq. iIntros ">H [Hw HE]". iApply "H"; by iFrame. Qed.
-
-Lemma bupd_fupd E P : (|==> P) ={E}=∗ P.
-Proof. rewrite uPred_fupd_eq. by iIntros ">? [$ $] !> !>". Qed.
-
-Lemma fupd_mono E1 E2 P Q : (P ⊢ Q) → (|={E1,E2}=> P) ⊢ |={E1,E2}=> Q.
-Proof.
-  rewrite uPred_fupd_eq. iIntros (HPQ) "HP HwE". rewrite -HPQ. by iApply "HP".
-Qed.
-
-Lemma fupd_trans E1 E2 E3 P : (|={E1,E2}=> |={E2,E3}=> P) ⊢ |={E1,E3}=> P.
-Proof.
-  rewrite uPred_fupd_eq. iIntros "HP HwE".
-  iMod ("HP" with "HwE") as ">(Hw & HE & HP)". iApply "HP"; by iFrame.
-Qed.
-
-Lemma fupd_mask_frame_r' E1 E2 Ef P :
-  E1 ## Ef → (|={E1,E2}=> ⌜E2 ## Ef⌝ → P) ={E1 ∪ Ef,E2 ∪ Ef}=∗ P.
-Proof.
-  intros. rewrite uPred_fupd_eq /uPred_fupd_def ownE_op //.
-  iIntros "Hvs (Hw & HE1 &HEf)".
-  iMod ("Hvs" with "[Hw HE1]") as ">($ & HE2 & HP)"; first by iFrame.
-  iDestruct (ownE_op' with "[HE2 HEf]") as "[? $]"; first by iFrame.
-  iIntros "!> !>". by iApply "HP".
-Qed.
-
-Lemma fupd_frame_r E1 E2 P Q : (|={E1,E2}=> P) ∗ Q ={E1,E2}=∗ P ∗ Q.
-Proof. rewrite uPred_fupd_eq /uPred_fupd_def. by iIntros "[HwP $]". Qed.
-
-Lemma fupd_plain' E1 E2 E2' P Q `{!Plain P} :
-  E1 ⊆ E2 →
-  (Q ={E1, E2'}=∗ P) -∗ (|={E1, E2}=> Q) ={E1}=∗ (|={E1, E2}=> Q) ∗ P.
-Proof.
-  iIntros ((E3&->&HE)%subseteq_disjoint_union_L) "HQP HQ".
-  rewrite uPred_fupd_eq /uPred_fupd_def ownE_op //. iIntros "H".
-  iMod ("HQ" with "H") as ">(Hws & [HE1 HE3] & HQ)"; iModIntro.
-  iAssert (◇ P)%I as "#HP".
-  { by iMod ("HQP" with "HQ [$]") as "(_ & _ & HP)". }
-  iMod "HP". iFrame. auto.
-Qed.
-
-Lemma later_fupd_plain E P `{!Plain P} : (▷ |={E}=> P) ={E}=∗ ▷ ◇ P.
-Proof.
-  rewrite uPred_fupd_eq /uPred_fupd_def. iIntros "HP [Hw HE]".
-  iAssert (▷ ◇ P)%I with "[-]" as "#$"; last by iFrame.
-  iNext. by iMod ("HP" with "[$]") as "(_ & _ & HP)".
-Qed.
-
-(** * Derived rules *)
-Global Instance fupd_mono' E1 E2 : Proper ((⊢) ==> (⊢)) (fupd E1 E2).
-Proof. intros P Q; apply fupd_mono. Qed.
-Global Instance fupd_flip_mono' E1 E2 :
-  Proper (flip (⊢) ==> flip (⊢)) (fupd E1 E2).
-Proof. intros P Q; apply fupd_mono. Qed.
-
-Lemma fupd_intro E P : P ={E}=∗ P.
-Proof. iIntros "HP". by iApply bupd_fupd. Qed.
-Lemma fupd_intro_mask' E1 E2 : E2 ⊆ E1 → (|={E1,E2}=> |={E2,E1}=> True)%I.
-Proof. exact: fupd_intro_mask. Qed.
-Lemma fupd_except_0 E1 E2 P : (|={E1,E2}=> ◇ P) ={E1,E2}=∗ P.
-Proof. by rewrite {1}(fupd_intro E2 P) except_0_fupd fupd_trans. Qed.
-
-Lemma fupd_frame_l E1 E2 P Q : (P ∗ |={E1,E2}=> Q) ={E1,E2}=∗ P ∗ Q.
-Proof. rewrite !(comm _ P); apply fupd_frame_r. Qed.
-Lemma fupd_wand_l E1 E2 P Q : (P -∗ Q) ∗ (|={E1,E2}=> P) ={E1,E2}=∗ Q.
-Proof. by rewrite fupd_frame_l wand_elim_l. Qed.
-Lemma fupd_wand_r E1 E2 P Q : (|={E1,E2}=> P) ∗ (P -∗ Q) ={E1,E2}=∗ Q.
-Proof. by rewrite fupd_frame_r wand_elim_r. Qed.
-
-Lemma fupd_trans_frame E1 E2 E3 P Q :
-  ((Q ={E2,E3}=∗ True) ∗ |={E1,E2}=> (Q ∗ P)) ={E1,E3}=∗ P.
-Proof.
-  rewrite fupd_frame_l assoc -(comm _ Q) wand_elim_r.
-  by rewrite fupd_frame_r left_id fupd_trans.
-Qed.
-
-Lemma fupd_mask_frame_r E1 E2 Ef P :
-  E1 ## Ef → (|={E1,E2}=> P) ={E1 ∪ Ef,E2 ∪ Ef}=∗ P.
-Proof.
-  iIntros (?) "H". iApply fupd_mask_frame_r'; auto.
-  iApply fupd_wand_r; iFrame "H"; eauto.
-Qed.
-Lemma fupd_mask_mono E1 E2 P : E1 ⊆ E2 → (|={E1}=> P) ={E2}=∗ P.
-Proof.
-  intros (Ef&->&?)%subseteq_disjoint_union_L. by apply fupd_mask_frame_r.
-Qed.
-
-Lemma fupd_sep E P Q : (|={E}=> P) ∗ (|={E}=> Q) ={E}=∗ P ∗ Q.
-Proof. by rewrite fupd_frame_r fupd_frame_l fupd_trans. Qed.
-Lemma fupd_big_sepL {A} E (Φ : nat → A → iProp Σ) (l : list A) :
-  ([∗ list] k↦x ∈ l, |={E}=> Φ k x) ={E}=∗ [∗ list] k↦x ∈ l, Φ k x.
-Proof.
-  apply (big_opL_forall (λ P Q, P ={E}=∗ Q)); auto using fupd_intro.
-  intros P1 P2 HP Q1 Q2 HQ. by rewrite HP HQ -fupd_sep.
-Qed.
-Lemma fupd_big_sepM `{Countable K} {A} E (Φ : K → A → iProp Σ) (m : gmap K A) :
-  ([∗ map] k↦x ∈ m, |={E}=> Φ k x) ={E}=∗ [∗ map] k↦x ∈ m, Φ k x.
-Proof.
-  apply (big_opM_forall (λ P Q, P ={E}=∗ Q)); auto using fupd_intro.
-  intros P1 P2 HP Q1 Q2 HQ. by rewrite HP HQ -fupd_sep.
-Qed.
-Lemma fupd_big_sepS `{Countable A} E (Φ : A → iProp Σ) X :
-  ([∗ set] x ∈ X, |={E}=> Φ x) ={E}=∗ [∗ set] x ∈ X, Φ x.
-Proof.
-  apply (big_opS_forall (λ P Q, P ={E}=∗ Q)); auto using fupd_intro.
-  intros P1 P2 HP Q1 Q2 HQ. by rewrite HP HQ -fupd_sep.
-Qed.
-
-Lemma fupd_plain E1 E2 P Q `{!Plain P} :
-  E1 ⊆ E2 → (Q -∗ P) -∗ (|={E1, E2}=> Q) ={E1}=∗ (|={E1, E2}=> Q) ∗ P.
-Proof.
-  iIntros (HE) "HQP HQ". iApply (fupd_plain' _ _ E1 with "[HQP] HQ"); first done.
-  iIntros "?". iApply fupd_intro. by iApply "HQP".
-Qed.
-End fupd.
-
-(** Proofmode class instances *)
-Section proofmode_classes.
-  Context `{invG Σ}.
-  Implicit Types P Q : iProp Σ.
-
-  Global Instance from_pure_fupd E P φ : FromPure P φ → FromPure (|={E}=> P) φ.
-  Proof. rewrite /FromPure. intros <-. apply fupd_intro. Qed.
-
-  Global Instance from_assumption_fupd E p P Q :
-    FromAssumption p P (|==> Q) → FromAssumption p P (|={E}=> Q)%I.
-  Proof. rewrite /FromAssumption=>->. apply bupd_fupd. Qed.
-
-  Global Instance into_wand_fupd E p q R P Q :
-    IntoWand false false R P Q →
-    IntoWand p q (|={E}=> R) (|={E}=> P) (|={E}=> Q).
-  Proof.
-    rewrite /IntoWand /= => HR. rewrite !affinely_persistently_if_elim HR.
-    apply wand_intro_l. by rewrite fupd_sep wand_elim_r.
-  Qed.
-
-  Global Instance into_wand_fupd_persistent E1 E2 p q R P Q :
-    IntoWand false q R P Q → IntoWand p q (|={E1,E2}=> R) P (|={E1,E2}=> Q).
-  Proof.
-    rewrite /IntoWand /= => HR. rewrite affinely_persistently_if_elim HR.
-    apply wand_intro_l. by rewrite fupd_frame_l wand_elim_r.
-  Qed.
-
-  Global Instance into_wand_fupd_args E1 E2 p q R P Q :
-    IntoWand p false R P Q → IntoWand' p q R (|={E1,E2}=> P) (|={E1,E2}=> Q).
-  Proof.
-    rewrite /IntoWand' /IntoWand /= => ->.
-    apply wand_intro_l. by rewrite affinely_persistently_if_elim fupd_wand_r.
-  Qed.
-
-  Global Instance from_sep_fupd E P Q1 Q2 :
-    FromSep P Q1 Q2 → FromSep (|={E}=> P) (|={E}=> Q1) (|={E}=> Q2).
-  Proof. rewrite /FromSep =><-. apply fupd_sep. Qed.
-
-  Global Instance from_or_fupd E1 E2 P Q1 Q2 :
-    FromOr P Q1 Q2 → FromOr (|={E1,E2}=> P) (|={E1,E2}=> Q1) (|={E1,E2}=> Q2).
-  Proof. rewrite /FromOr=><-. apply or_elim; apply fupd_mono; auto with I. Qed.
-
-  Global Instance from_exist_fupd {A} E1 E2 P (Φ : A → iProp Σ) :
-    FromExist P Φ → FromExist (|={E1,E2}=> P) (λ a, |={E1,E2}=> Φ a)%I.
-  Proof.
-    rewrite /FromExist=><-. apply exist_elim=> a. by rewrite -(exist_intro a).
-  Qed.
-
-  Global Instance frame_fupd p E1 E2 R P Q :
-    Frame p R P Q → Frame p R (|={E1,E2}=> P) (|={E1,E2}=> Q).
-  Proof. rewrite /Frame=><-. by rewrite fupd_frame_l. Qed.
-
-  Global Instance is_except_0_fupd E1 E2 P : IsExcept0 (|={E1,E2}=> P).
-  Proof. by rewrite /IsExcept0 except_0_fupd. Qed.
-
-  Global Instance from_modal_fupd E P : FromModal (|={E}=> P) P.
-  Proof. rewrite /FromModal. apply fupd_intro. Qed.
-
-  Global Instance elim_modal_bupd_fupd E1 E2 P Q :
-    ElimModal (|==> P) P (|={E1,E2}=> Q) (|={E1,E2}=> Q).
-  Proof.
-    by rewrite /ElimModal (bupd_fupd E1) fupd_frame_r wand_elim_r fupd_trans.
-  Qed.
-  Global Instance elim_modal_fupd_fupd E1 E2 E3 P Q :
-    ElimModal (|={E1,E2}=> P) P (|={E1,E3}=> Q) (|={E2,E3}=> Q).
-  Proof. by rewrite /ElimModal fupd_frame_r wand_elim_r fupd_trans. Qed.
-
-  Global Instance add_modal_fupd E1 E2 P Q :
-    AddModal (|={E1}=> P) P (|={E1,E2}=> Q).
-  Proof. by rewrite /AddModal fupd_frame_r wand_elim_r fupd_trans. Qed.
-End proofmode_classes.
-
-Hint Extern 2 (coq_tactics.envs_entails _ (|={_}=> _)) => iModIntro.
-
-(** Fancy updates that take a step. *)
-
-Section step_fupd.
-Context `{invG Σ}.
-
-Lemma step_fupd_wand E1 E2 P Q : (|={E1,E2}▷=> P) -∗ (P -∗ Q) -∗ |={E1,E2}▷=> Q.
-Proof. iIntros "HP HPQ". by iApply "HPQ". Qed.
-
-Lemma step_fupd_mask_frame_r E1 E2 Ef P :
-  E1 ## Ef → E2 ## Ef → (|={E1,E2}▷=> P) ⊢ |={E1 ∪ Ef,E2 ∪ Ef}▷=> P.
-Proof.
-  iIntros (??) "HP". iApply fupd_mask_frame_r. done. iMod "HP". iModIntro.
-  iNext. by iApply fupd_mask_frame_r.
-Qed.
-
-Lemma step_fupd_mask_mono E1 E2 F1 F2 P :
-  F1 ⊆ F2 → E1 ⊆ E2 → (|={E1,F2}▷=> P) ⊢ |={E2,F1}▷=> P.
-Proof.
-  iIntros (??) "HP".
-  iMod (fupd_intro_mask') as "HM1"; first done. iMod "HP".
-  iMod (fupd_intro_mask') as "HM2"; first done. iModIntro.
-  iNext. iMod "HM2". iMod "HP". iMod "HM1". done.
-Qed.
-
-Lemma step_fupd_intro E1 E2 P : E2 ⊆ E1 → ▷ P -∗ |={E1,E2}▷=> P.
-Proof. iIntros (?) "HP". iApply (step_fupd_mask_mono E2 _ _ E2); auto. Qed.
-End step_fupd.
